Some reordering and renaming

proof/TPOSR/CtxCoercion.v
@@ -1,14 +1,13 @@
-Require Import Lambda.Tactics.
-Require Import Lambda.Utils.
-
 Require Import Lambda.TPOSR.Terms.
 Require Import Lambda.TPOSR.Reduction.
 Require Import Lambda.TPOSR.Conv.
 Require Import Lambda.TPOSR.LiftSubst.
 Require Import Lambda.TPOSR.Env.
-Require Import Lambda.TPOSR.TypesNoDerivs.
-Require Import Lambda.TPOSR.Thinning.
+Require Import Lambda.TPOSR.Types.
+Require Import Lambda.TPOSR.Basic.
+Require Import Lambda.TPOSR.CtxCoercion.
 Require Import Lambda.TPOSR.LeftReflexivity.
+Require Import Lambda.TPOSR.RightReflexivity.
 
 Set Implicit Arguments.
 
@@ -18,302 +17,65 @@ Implicit Types A B M N T t u v : lterm.
 Implicit Types e f g : lenv.
 
 Inductive coerce_in_env : lenv -> lenv -> Prop :=
-  | coerce_env_hd : forall e t u s, e |-- t >-> u : s -> e |-- t -> t : s -> e |-- u -> u : Srt_l s ->
-	coerce_in_env (t :: e) (u :: e)
+  | coerce_env_hd : forall e t u s, e |-- t >-> u : s -> 
+	coerce_in_env (u :: e) (t :: e)
   | coerce_env_tl :
-      forall e f t, coerce_in_env e f -> 
-      forall s, f |-- t -> t : Srt_l s ->
-      coerce_in_env (t :: e) (t :: f).
+        forall e f t, tposr_wf (t :: f) -> coerce_in_env e f -> coerce_in_env (t :: e) (t :: f).
 
 Hint Resolve coerce_env_hd coerce_env_tl: coc.
 
-Lemma coerce_item :
-   forall n t e,
-   item_llift t e n ->
-   forall f, coerce_in_env e f ->
-   item_llift t f n \/
-   ((forall g, trunc _ (S n) e g -> trunc _ (S n) f g) /\
-   exists u, item_llift u f n /\ (exists s : sort, f |-- t >-> u : s /\ f |-- u -> u : s)).
-simple induction n.
-do 3 intro.
-elim H.
-do 4 intro.
-rewrite H0.
-inversion_clear H1.
-intros.
-inversion_clear H1.
-right.
-split; intros.
-inversion_clear H1; auto with coc core arith datatypes.
+Lemma coerce_in_env_pre : forall e f, coerce_in_env e f -> CtxCoercion.
 
-exists (llift 1 u).
-split.
-inversion_clear H.
 
-unfold item_llift.
-exists u; auto with coc core arith datatypes.
-
-exists s ; auto with coc core.
-change (Srt_l s) with (llift 1 (Srt_l s)).
-split.
-apply thinning_n_coerce with l ; auto with coc core ;
-apply wf_cons with s ; eauto with coc.
-apply thinning_n with l ; auto with coc core ;
-apply wf_cons with s ; auto.
-
-left.
-exists x; auto with coc core arith datatypes.
-
-do 5 intro.
-elim H0.
-do 4 intro.
-rewrite H1.
-inversion_clear H2.
-intros.
-inversion_clear H2.
-left.
-exists x; auto with coc core arith datatypes.
-
-elim H with (llift (S n0) x) l f0; auto with coc core arith datatypes; intros.
-left.
-elim H2; intros.
-exists x0; auto with coc core arith datatypes.
-rewrite simpl_llift.
-pattern (llift (S (S n0)) x0) in |- *.
-rewrite simpl_llift.
-rewrite H6; auto with coc core arith datatypes.
-
-right.
-elim H2.
-clear H2.
-simple induction 2; intros.
-clear H7.
-split; intros.
-inversion_clear H7; auto with coc core arith datatypes.
-
-destruct H6.
-destruct H6.
-destruct H7.
-unfold item_llift.
-exists (llift 1 x1).
-split ; auto with coc core.
-inversion_clear H6 ; auto with coc core arith.
-exists x3.
-rewrite H8.
-rewrite <- simpl_llift.
-auto with coc core.
-auto with coc.
-
-exists x2.
-pattern (llift (S (S n0)) x) ; rewrite simpl_llift.
-change (Srt_l x2) with (llift 1 (Srt_l x2)).
-destruct H7.
-split.
-eapply thinning_n_coerce ; auto with coc core ;
-apply wf_cons with s ; auto.
-eapply thinning_n ; auto with coc core ;
-apply wf_cons with s ; auto.
-
-exists x; auto with coc core arith datatypes.
-Qed.
-
-Lemma ind_coerce_env :
-  (forall e t u T, e |-- t -> u : T -> 
-  forall f, coerce_in_env e f -> f |-- t -> u : T) /\
-  (forall e, tposr_wf e -> 
-  forall f, coerce_in_env e f -> tposr_wf f) /\
-  (forall e t u s, e |-- t ~= u : s -> 
-  forall f, coerce_in_env e f -> f |-- t ~= u : s) /\
-  (forall e t u s, e |-- t >-> u : s -> 
-  forall f, coerce_in_env e f -> f |-- t >-> u : s).
-Proof.
-  apply ind_tposr_wf_eq_coerce with
-  (P:=fun e t u T => fun H : e |-- t -> u : T => 
-  forall f, coerce_in_env e f -> f |-- t -> u : T) 
-  (P0:=fun e => fun H : tposr_wf e => 
-  forall f, coerce_in_env e f -> tposr_wf f) 
-  (P1:=fun e t u s => fun H : e |-- t ~= u : s => 
-  forall f, coerce_in_env e f -> f |-- t ~= u : s) 
-  (P2:=fun e t u s => fun H : e |-- t >-> u : s => 
-  forall f, coerce_in_env e f -> f |-- t >-> u : s) ;
-  intros ; 
-auto with coc core arith datatypes.
-
-destruct (coerce_item i H0) ; destruct_exists.
-apply tposr_var ; auto with coc.
-apply tposr_conv with x x0.
-apply tposr_var.
-apply (H _ H0).
-assumption.
-apply tposr_coerce_sym.
-assumption.
-
-apply tposr_prod with s1 ; eauto with coc.
-
-apply tposr_abs with s1 B' s2 ; eauto with coc.
-
-apply tposr_app with A A' s1 s2 ; eauto with coc.
-
-apply tposr_beta with A' s1 B' s2 ; eauto with coc.
-
-apply tposr_conv with A s ; auto with coc.
-
-apply tposr_subset ; eauto with coc.
-
-apply tposr_sum with s1 s2 ; eauto with coc.
-
-apply tposr_pair with s1 s2 s3 ; eauto with coc.
-
-apply tposr_pi1 with s1 s2 s3 ; eauto with coc.
-
-eapply tposr_pi1_red ; eauto with coc.
-
-apply tposr_pi2 with s1 s2 s3 ; eauto with coc.
-
-eapply tposr_pi2_red  ; eauto with coc.
-
-inversion H.
-inversion H0.
-subst.
-apply wf_cons with s0 ; auto.
-apply wf_cons with s0 ; auto.
-
-apply tposr_eq_trans with X ; auto with coc.
-
-apply tposr_coerce_prod with s ; eauto with coc.
-
-apply tposr_coerce_sum with s s' ; eauto with coc.
-
-apply tposr_coerce_sub_l  ; eauto with coc.
-
-apply tposr_coerce_sub_r  ; eauto with coc.
-
-apply tposr_coerce_trans with B ; auto with coc.
-Qed.
-
-Lemma tposr_coerce_env : forall e t u T, e |-- t -> u : T -> 
+Lemma type_coerce_env : forall e t u T, e |-- t -> u : T -> 
   forall f, coerce_in_env e f -> f |-- t -> u : T.
-Proof (proj1 ind_coerce_env).
+Proof (proj1 ind_conv_env).
 
-Lemma eq_coerce_env : forall e u v s, e |-- u ~= v : s ->
-  forall f, coerce_in_env e f -> f |-- u ~= v : s.
-Proof (proj1 (proj2 (proj2 ind_coerce_env))).
+Lemma eq_coerce_env : forall e T U s, e |-- T ~= U : s -> 
+  forall f, coerce_in_env e f -> f |-- T ~= U : s.
+Proof (proj1 (proj2 (proj2 ind_conv_env))).
 
 Lemma coerce_coerce_env : forall e T U s, e |-- T >-> U : s -> 
   forall f, coerce_in_env e f -> f |-- T >-> U : s.
-Proof (proj2 (proj2 (proj2 ind_coerce_env))).
+Proof (proj2 (proj2 (proj2 ind_conv_env))).
 
-Hint Resolve tposr_coerce_env eq_coerce_env coerce_coerce_env : ecoc.
-
-Inductive coerce_in_env_full : lenv -> lenv -> Prop :=
-  | coerce_env_trans : forall e f g, coerce_in_env_full e f -> coerce_in_env_full f g -> coerce_in_env_full e g
-  | coerce_env_in_env : forall e f, coerce_in_env e f -> coerce_in_env_full e f
-  | coerce_env_nil : coerce_in_env_full nil nil.
-
-Hint Resolve coerce_env_in_env coerce_env_nil : coc.
-
-Lemma coerce_env_sym : forall e f, coerce_in_env e f -> coerce_in_env f e.
+Corollary tposrp_coerce_env : forall e t u T, e |-- t -+> u : T -> 
+  forall f, coerce_in_env e f -> f |-- t -+> u : T.
 Proof.
   induction 1 ; simpl ; intros ; auto with coc.
-  apply coerce_env_hd with s ; eauto with coc.
-  apply coerce_env_tl with s ; eauto with coc.
-  apply tposr_coerce_env with f ; auto.
-Qed.  
-
-Lemma coerce_env_full_sym : forall e f, coerce_in_env_full e f -> coerce_in_env_full f e.
-Proof.
-  induction 1 ; simpl ; intros ; eauto with coc.
-  apply coerce_env_trans with f ; auto.
-  apply coerce_env_in_env ; auto.
-  apply coerce_env_sym ; auto.
-Qed.
-
-Hint Resolve coerce_env_sym coerce_env_full_sym : coc.
-
-Lemma coerce_env_full :
-  (forall e t u T, e |-- t -> u : T -> 
-  forall f, coerce_in_env_full e f -> f |-- t -> u : T).
-Proof.
-  intros.
-  induction H0 ; auto.
-
-  apply tposr_coerce_env with e ; auto with coc.
-Qed.
-
-Lemma coerce_env_full_cons : forall G D, coerce_in_env_full G D -> forall T, tposr_wf (T :: G) ->
-  coerce_in_env_full (T :: G) (T :: D).
-Proof.
-  induction 1 ; simpl ; intros.
-  apply coerce_env_trans with (T :: f) ; eauto with coc.
-  apply IHcoerce_in_env_full2.
-  inversion H1.
-  apply wf_cons with  s.
-  apply coerce_env_full with e ; auto with coc.
-
-  inversion H0.
-  subst.
-  apply coerce_env_in_env ; eauto with coc.
-
-  apply coerce_env_in_env ; auto with coc.
-  inversion H.
-  assert(nil |-- T -> T : s).
-  eauto with coc.
-  apply coerce_env_hd with s ; auto with coc.
-Qed.
-
-Corollary tposrp_coerce_env_full : 
-  (forall e t u T, e |-- t -+> u : T -> 
-  forall f, coerce_in_env_full e f -> f |-- t -+> u : T).
-Proof.
-  induction 1 ; simpl ; intros ; auto with coc.
-  apply tposrp_tposr ; eapply coerce_env_full ; eauto with coc.
+  apply tposrp_tposr.
+  eapply type_coerce_env ; eauto with coc.
   apply tposrp_trans with X ; auto with coc.
 Qed.
 
-Corollary eq_coerce_env_full : 
-  (forall e t u s, e |-- t ~= u : s -> 
-  forall f, coerce_in_env_full e f -> f |-- t ~= u : s).
+Hint Resolve type_coerce_env eq_coerce_env coerce_coerce_env : ecoc.
+
+Lemma coerce_in_env_sym : forall e f, coerce_in_env e f -> coerce_in_env f e.
 Proof.
   induction 1 ; simpl ; intros ; auto with coc.
-  apply tposr_eq_tposr ; eapply coerce_env_full ; eauto with coc.
-  apply tposr_eq_trans with X ; auto with coc.
+  apply coerce_env_hd with s ; auto with coc.
+  apply coerce_env_tl ; auto with coc.
+  inversion H.
+  subst.
+  apply wf_cons with A' s.
+  apply type_coerce_env with f ; auto with coc.
 Qed.
 
-Hint Resolve coerce_env_full eq_coerce_env_full : ecoc.
+Hint Resolve coerce_in_env_sym : coc.
 
-Corollary coerce_coerce_env_full : 
-  (forall e t u s, e |-- t >-> u : s -> 
-  forall f, coerce_in_env_full e f -> f |-- t >-> u : s).
+Require Import Lambda.TPOSR.Substitution.
+
+Lemma substitution_coerce_tposrp : 
+  forall e d d' t, e |-- d -+> d' : t -> 
+  forall u v s, t :: e |-- u >-> v : s -> e |-- (lsubst d u) >-> (lsubst d' v) : s.
 Proof.
-  induction 1 ; simpl ; intros ; auto with coc.
-
-  apply tposr_coerce_conv ; eapply eq_coerce_env_full ; eauto with coc.
-
-  assert(coerce_in_env_full (A' :: e) (A' :: f)) by
-  (apply coerce_env_full_cons ; auto with coc;
-  eauto with coc ecoc).
-  assert(coerce_in_env_full (A :: e) (A :: f)) by
-  (apply coerce_env_full_cons ; auto with coc;
-  eauto with coc ecoc).
-  apply tposr_coerce_prod with s ; eauto with coc ecoc.
-
-  assert(coerce_in_env_full (A' :: e) (A' :: f)) by
-  (apply coerce_env_full_cons ; auto with coc;
-  eauto with coc ecoc).
-  assert(coerce_in_env_full (A :: e) (A :: f)) by
-  (apply coerce_env_full_cons ; auto with coc;
-  eauto with coc ecoc).
-  apply tposr_coerce_sum with s s' ; eauto with coc ecoc.
-
-  assert(coerce_in_env_full (U :: e) (U :: f)) by
-  (apply coerce_env_full_cons ; auto with coc;
-  eauto with coc ecoc).
-  apply tposr_coerce_sub_l ; eauto with coc ecoc.
-
-  assert(coerce_in_env_full (U' :: e) (U' :: f)) by
-  (apply coerce_env_full_cons ; auto with coc ; eauto with coc ecoc).
-  apply tposr_coerce_sub_r ; eauto with coc ecoc.
+  induction 1 ; intros.
   
-  apply tposr_coerce_trans with B ; auto.
+  apply substitution_coerce with Z ; auto.
+  apply tposr_coerce_trans with (lsubst X u) ; auto.
+  apply IHtposrp1.
+  apply tposr_coerce_conv ; apply tposr_eq_tposr ; auto.
+  apply (coerce_refl_l H1).
 Qed.
+
 
