proof/TPOSR/LeftReflexivity.v
@@ -3,7 +3,7 @@ Require Import Lambda.TPOSR.Reduction.
 Require Import Lambda.TPOSR.Conv.
 Require Import Lambda.TPOSR.LiftSubst.
 Require Import Lambda.TPOSR.Env.
-Require Import Lambda.TPOSR.TypesNoDerivs.
+Require Import Lambda.TPOSR.Types.
 
 Set Implicit Arguments.
 
@@ -60,8 +60,7 @@ Proof.
 
   apply tposr_pi1 with s1 s2 s3 ; eauto with coc ecoc.
 
-  apply tposr_pi1 with s1 s2 s3; auto with coc ecoc.
-  eauto with coc ecoc.
+  apply tposr_pi1 with s1 s2 s3; eauto with coc ecoc.
 
   apply tposr_pi2 with s1 s2 s3 ; eauto with coc ecoc.
 
