proof/TPOSR/PreCtxCoercion.v
@@ -1,0 +1,319 @@
+Require Import Lambda.Tactics.
+Require Import Lambda.Utils.
+
+Require Import Lambda.TPOSR.Terms.
+Require Import Lambda.TPOSR.Reduction.
+Require Import Lambda.TPOSR.Conv.
+Require Import Lambda.TPOSR.LiftSubst.
+Require Import Lambda.TPOSR.Env.
+Require Import Lambda.TPOSR.Types.
+Require Import Lambda.TPOSR.Thinning.
+Require Import Lambda.TPOSR.LeftReflexivity.
+
+Set Implicit Arguments.
+
+Implicit Types i k m n p : nat.
+Implicit Type s : sort.
+Implicit Types A B M N T t u v : lterm.
+Implicit Types e f g : lenv.
+
+Inductive pre_coerce_in_env : lenv -> lenv -> Prop :=
+  | pre_coerce_env_hd : forall e t u s, e |-- t >-> u : s -> e |-- t -> t : s -> e |-- u -> u : Srt_l s ->
+	pre_coerce_in_env (t :: e) (u :: e)
+  | pre_coerce_env_tl :
+      forall e f t, pre_coerce_in_env e f -> 
+      forall s, f |-- t -> t : Srt_l s ->
+      pre_coerce_in_env (t :: e) (t :: f).
+
+Hint Resolve pre_coerce_env_hd pre_coerce_env_tl: coc.
+
+Lemma coerce_item :
+   forall n t e,
+   item_llift t e n ->
+   forall f, pre_coerce_in_env e f ->
+   item_llift t f n \/
+   ((forall g, trunc _ (S n) e g -> trunc _ (S n) f g) /\
+   exists u, item_llift u f n /\ (exists s : sort, f |-- t >-> u : s /\ f |-- u -> u : s)).
+simple induction n.
+do 3 intro.
+elim H.
+do 4 intro.
+rewrite H0.
+inversion_clear H1.
+intros.
+inversion_clear H1.
+right.
+split; intros.
+inversion_clear H1; auto with coc core arith datatypes.
+
+exists (llift 1 u).
+split.
+inversion_clear H.
+
+unfold item_llift.
+exists u; auto with coc core arith datatypes.
+
+exists s ; auto with coc core.
+change (Srt_l s) with (llift 1 (Srt_l s)).
+split.
+apply thinning_n_coerce with l ; auto with coc core ;
+apply wf_cons with s ; eauto with coc.
+apply thinning_n with l ; auto with coc core ;
+apply wf_cons with s ; auto.
+
+left.
+exists x; auto with coc core arith datatypes.
+
+do 5 intro.
+elim H0.
+do 4 intro.
+rewrite H1.
+inversion_clear H2.
+intros.
+inversion_clear H2.
+left.
+exists x; auto with coc core arith datatypes.
+
+elim H with (llift (S n0) x) l f0; auto with coc core arith datatypes; intros.
+left.
+elim H2; intros.
+exists x0; auto with coc core arith datatypes.
+rewrite simpl_llift.
+pattern (llift (S (S n0)) x0) in |- *.
+rewrite simpl_llift.
+rewrite H6; auto with coc core arith datatypes.
+
+right.
+elim H2.
+clear H2.
+simple induction 2; intros.
+clear H7.
+split; intros.
+inversion_clear H7; auto with coc core arith datatypes.
+
+destruct H6.
+destruct H6.
+destruct H7.
+unfold item_llift.
+exists (llift 1 x1).
+split ; auto with coc core.
+inversion_clear H6 ; auto with coc core arith.
+exists x3.
+rewrite H8.
+rewrite <- simpl_llift.
+auto with coc core.
+auto with coc.
+
+exists x2.
+pattern (llift (S (S n0)) x) ; rewrite simpl_llift.
+change (Srt_l x2) with (llift 1 (Srt_l x2)).
+destruct H7.
+split.
+eapply thinning_n_coerce ; auto with coc core ;
+apply wf_cons with s ; auto.
+eapply thinning_n ; auto with coc core ;
+apply wf_cons with s ; auto.
+
+exists x; auto with coc core arith datatypes.
+Qed.
+
+Lemma ind_pre_coerce_env :
+  (forall e t u T, e |-- t -> u : T -> 
+  forall f, pre_coerce_in_env e f -> f |-- t -> u : T) /\
+  (forall e, tposr_wf e -> 
+  forall f, pre_coerce_in_env e f -> tposr_wf f) /\
+  (forall e t u s, e |-- t ~= u : s -> 
+  forall f, pre_coerce_in_env e f -> f |-- t ~= u : s) /\
+  (forall e t u s, e |-- t >-> u : s -> 
+  forall f, pre_coerce_in_env e f -> f |-- t >-> u : s).
+Proof.
+  apply ind_tposr_wf_eq_coerce with
+  (P:=fun e t u T => fun H : e |-- t -> u : T => 
+  forall f, pre_coerce_in_env e f -> f |-- t -> u : T) 
+  (P0:=fun e => fun H : tposr_wf e => 
+  forall f, pre_coerce_in_env e f -> tposr_wf f) 
+  (P1:=fun e t u s => fun H : e |-- t ~= u : s => 
+  forall f, pre_coerce_in_env e f -> f |-- t ~= u : s) 
+  (P2:=fun e t u s => fun H : e |-- t >-> u : s => 
+  forall f, pre_coerce_in_env e f -> f |-- t >-> u : s) ;
+  intros ; 
+auto with coc core arith datatypes.
+
+destruct (coerce_item i H0) ; destruct_exists.
+apply tposr_var ; auto with coc.
+apply tposr_conv with x x0.
+apply tposr_var.
+apply (H _ H0).
+assumption.
+apply tposr_coerce_sym.
+assumption.
+
+apply tposr_prod with s1 ; eauto with coc.
+
+apply tposr_abs with s1 B' s2 ; eauto with coc.
+
+apply tposr_app with A A' s1 s2 ; eauto with coc.
+
+apply tposr_beta with A' s1 B' s2 ; eauto with coc.
+
+apply tposr_conv with A s ; auto with coc.
+
+apply tposr_subset ; eauto with coc.
+
+apply tposr_sum with s1 s2 ; eauto with coc.
+
+apply tposr_pair with s1 s2 s3 ; eauto with coc.
+
+apply tposr_pi1 with s1 s2 s3 ; eauto with coc.
+
+eapply tposr_pi1_red ; eauto with coc.
+
+apply tposr_pi2 with s1 s2 s3 ; eauto with coc.
+
+eapply tposr_pi2_red  ; eauto with coc.
+
+inversion H.
+inversion H0.
+subst.
+apply wf_cons with s0 ; auto.
+apply wf_cons with s0 ; auto.
+
+apply tposr_eq_trans with X ; auto with coc.
+
+apply tposr_coerce_prod with s ; eauto with coc.
+
+apply tposr_coerce_sum with s s' ; eauto with coc.
+
+apply tposr_coerce_sub_l  ; eauto with coc.
+
+apply tposr_coerce_sub_r  ; eauto with coc.
+
+apply tposr_coerce_trans with B ; auto with coc.
+Qed.
+
+Lemma tposr_pre_coerce_env : forall e t u T, e |-- t -> u : T -> 
+  forall f, pre_coerce_in_env e f -> f |-- t -> u : T.
+Proof (proj1 ind_pre_coerce_env).
+
+Lemma eq_pre_coerce_env : forall e u v s, e |-- u ~= v : s ->
+  forall f, pre_coerce_in_env e f -> f |-- u ~= v : s.
+Proof (proj1 (proj2 (proj2 ind_pre_coerce_env))).
+
+Lemma coerce_pre_coerce_env : forall e T U s, e |-- T >-> U : s -> 
+  forall f, pre_coerce_in_env e f -> f |-- T >-> U : s.
+Proof (proj2 (proj2 (proj2 ind_pre_coerce_env))).
+
+Hint Resolve tposr_pre_coerce_env eq_pre_coerce_env coerce_pre_coerce_env : ecoc.
+
+Inductive pre_coerce_in_env_full : lenv -> lenv -> Prop :=
+  | pre_coerce_env_trans : forall e f g, pre_coerce_in_env_full e f -> pre_coerce_in_env_full f g -> pre_coerce_in_env_full e g
+  | pre_coerce_env_in_env : forall e f, pre_coerce_in_env e f -> pre_coerce_in_env_full e f
+  | pre_coerce_env_nil : pre_coerce_in_env_full nil nil.
+
+Hint Resolve pre_coerce_env_in_env pre_coerce_env_nil : coc.
+
+Lemma pre_coerce_env_sym : forall e f, pre_coerce_in_env e f -> pre_coerce_in_env f e.
+Proof.
+  induction 1 ; simpl ; intros ; auto with coc.
+  apply pre_coerce_env_hd with s ; eauto with coc.
+  apply pre_coerce_env_tl with s ; eauto with coc.
+  apply tposr_pre_coerce_env with f ; auto.
+Qed.  
+
+Lemma pre_coerce_env_full_sym : forall e f, pre_coerce_in_env_full e f -> pre_coerce_in_env_full f e.
+Proof.
+  induction 1 ; simpl ; intros ; eauto with coc.
+  apply pre_coerce_env_trans with f ; auto.
+  apply pre_coerce_env_in_env ; auto.
+  apply pre_coerce_env_sym ; auto.
+Qed.
+
+Hint Resolve pre_coerce_env_sym pre_coerce_env_full_sym : coc.
+
+Lemma pre_coerce_env_full :
+  (forall e t u T, e |-- t -> u : T -> 
+  forall f, pre_coerce_in_env_full e f -> f |-- t -> u : T).
+Proof.
+  intros.
+  induction H0 ; auto.
+
+  apply tposr_pre_coerce_env with e ; auto with coc.
+Qed.
+
+Lemma pre_coerce_env_full_cons : forall G D, pre_coerce_in_env_full G D -> forall T, tposr_wf (T :: G) ->
+  pre_coerce_in_env_full (T :: G) (T :: D).
+Proof.
+  induction 1 ; simpl ; intros.
+  apply pre_coerce_env_trans with (T :: f) ; eauto with coc.
+  apply IHpre_coerce_in_env_full2.
+  inversion H1.
+  apply wf_cons with  s.
+  apply pre_coerce_env_full with e ; auto with coc.
+
+  inversion H0.
+  subst.
+  apply pre_coerce_env_in_env ; eauto with coc.
+
+  apply pre_coerce_env_in_env ; auto with coc.
+  inversion H.
+  assert(nil |-- T -> T : s).
+  eauto with coc.
+  apply pre_coerce_env_hd with s ; auto with coc.
+Qed.
+
+Corollary tposrp_pre_coerce_env_full : 
+  (forall e t u T, e |-- t -+> u : T -> 
+  forall f, pre_coerce_in_env_full e f -> f |-- t -+> u : T).
+Proof.
+  induction 1 ; simpl ; intros ; auto with coc.
+  apply tposrp_tposr ; eapply pre_coerce_env_full ; eauto with coc.
+  apply tposrp_trans with X ; auto with coc.
+Qed.
+
+Corollary eq_pre_coerce_env_full : 
+  (forall e t u s, e |-- t ~= u : s -> 
+  forall f, pre_coerce_in_env_full e f -> f |-- t ~= u : s).
+Proof.
+  induction 1 ; simpl ; intros ; auto with coc.
+  apply tposr_eq_tposr ; eapply pre_coerce_env_full ; eauto with coc.
+  apply tposr_eq_trans with X ; auto with coc.
+Qed.
+
+Hint Resolve pre_coerce_env_full eq_pre_coerce_env_full : ecoc.
+
+Corollary coerce_pre_coerce_env_full : 
+  (forall e t u s, e |-- t >-> u : s -> 
+  forall f, pre_coerce_in_env_full e f -> f |-- t >-> u : s).
+Proof.
+  induction 1 ; simpl ; intros ; auto with coc.
+
+  apply tposr_coerce_conv ; eapply eq_pre_coerce_env_full ; eauto with coc.
+
+  assert(pre_coerce_in_env_full (A' :: e) (A' :: f)) by
+  (apply pre_coerce_env_full_cons ; auto with coc;
+  eauto with coc ecoc).
+  assert(pre_coerce_in_env_full (A :: e) (A :: f)) by
+  (apply pre_coerce_env_full_cons ; auto with coc;
+  eauto with coc ecoc).
+  apply tposr_coerce_prod with s ; eauto with coc ecoc.
+
+  assert(pre_coerce_in_env_full (A' :: e) (A' :: f)) by
+  (apply pre_coerce_env_full_cons ; auto with coc;
+  eauto with coc ecoc).
+  assert(pre_coerce_in_env_full (A :: e) (A :: f)) by
+  (apply pre_coerce_env_full_cons ; auto with coc;
+  eauto with coc ecoc).
+  apply tposr_coerce_sum with s s' ; eauto with coc ecoc.
+
+  assert(pre_coerce_in_env_full (U :: e) (U :: f)) by
+  (apply pre_coerce_env_full_cons ; auto with coc;
+  eauto with coc ecoc).
+  apply tposr_coerce_sub_l ; eauto with coc ecoc.
+
+  assert(pre_coerce_in_env_full (U' :: e) (U' :: f)) by
+  (apply pre_coerce_env_full_cons ; auto with coc ; eauto with coc ecoc).
+  apply tposr_coerce_sub_r ; eauto with coc ecoc.
+  
+  apply tposr_coerce_trans with B ; auto.
+Qed.
+
