proof/TPOSR/Thinning.v
@@ -3,7 +3,7 @@ Require Import Lambda.TPOSR.Reduction.
 Require Import Lambda.TPOSR.LiftSubst.
 Require Import Lambda.TPOSR.Env.
 Require Import Lambda.TPOSR.Conv.
-Require Import Lambda.TPOSR.TypesNoDerivs.
+Require Import Lambda.TPOSR.Types.
 Require Import Lambda.TPOSR.LeftReflexivity.
 
 Set Implicit Arguments.
@@ -93,12 +93,8 @@ apply H1 ; eauto with coc.
 apply wf_cons with s1 ; eauto with coc.
 
 assert (tposr_wf (llift_rec 1 A0 n :: f)) by (apply wf_cons with s1 ; eauto with coc).
-apply tposr_pi1_red with s1 s2 s3 (llift_rec 1 A'' n) (llift_rec 1 B'' (S n)) (llift_rec 1 v' n) ; auto with coc.
+apply tposr_pi1_red with (llift_rec 1 A' n) s1 (llift_rec 1 B' (S n)) s2 s3 (llift_rec 1 v' n) ; eauto with coc ecoc.
 
-(*apply tposr_pi1_red with (llift_rec 1 A' n) s1 (llift_rec 1 B' (S n))  s2 s3 (llift_rec 1 v' n); auto with coc.
-rewrite <- distr_llift_lsubst.
-auto with coc.
-*)
 assert (tposr_wf (llift_rec 1 A0 n :: f)) by (apply wf_cons with s1 ; eauto with coc).
 rewrite distr_llift_lsubst.
 simpl.
@@ -107,17 +103,11 @@ apply tposr_pi2 with s1 s2 s3 ; auto with coc.
 assert (tposr_wf (llift_rec 1 A0 n :: f)) by (apply wf_cons with s1 ; eauto with coc).
 rewrite distr_llift_lsubst.
 simpl.
-apply tposr_pi2_red with s1 s2 s3 (llift_rec 1 A'' n) (llift_rec 1 B'' (S n)) (llift_rec 1 u' n) ; auto with coc.
-(*
-apply tposr_pi2_red with (llift_rec 1 A' n) s1 (llift_rec 1 B' (S n))  s2 s3 (llift_rec 1 u' n); auto with coc.
-rewrite <- distr_llift_lsubst.
-auto with coc.
-*)
+apply tposr_pi2_red with (llift_rec 1 A' n) s1 (llift_rec 1 B' (S n)) s2 s3 (llift_rec 1 u' n) ; eauto with coc ecoc.
+
 apply tposr_eq_trans with (llift_rec 1 X n) ; auto with coc.
 
-
 apply tposr_coerce_prod with s ; eauto with coc ecoc.
-
 
 apply tposr_coerce_sum with s s' ; eauto with coc ecoc.
 
